significant developments in JsRecord

NS/JsRecord.v
@@ -5,6 +5,7 @@ Require Import Coq.Arith.PeanoNat.
 Require Import Coq.Arith.EqNat.
 Require Import Coq.Bool.Bool.
 Require Import Coq.Logic.FunctionalExtensionality.
+Require Import Coq.Relations.Relation_Definitions.
 From NS Require Import Misc.
 
 Notation js_record A := (list (string * A)).
@@ -57,13 +58,24 @@ Inductive JsRecordEqKeys0 {A: Type}: js_record A -> js_record A -> Prop :=
 .
 
 Inductive JsRecordAdd {A: Type} (kx: string) (vx: A) : js_record A -> js_record A -> Prop :=
-| JsRecordAdd_head : forall (xs: js_record A), JsRecordAdd kx vx xs ((kx, vx) :: xs)%list
+| JsRecordAdd_head : forall (xs: js_record A), ~JsRecordHasKey kx xs -> JsRecordAdd kx vx xs ((kx, vx) :: xs)%list
 | JsRecordAdd_cons : forall (kx0: string) (vx0: A) (xs xs': js_record A), kx0 <> kx -> JsRecordAdd kx vx xs xs' -> JsRecordAdd kx vx ((kx0, vx0) :: xs)%list ((kx0, vx0) :: xs')%list
+.
+
+Inductive JsRecordRel {A: Type} (rel: relation A): relation (js_record A) :=
+| JsRecordRel_nil : JsRecordRel rel nil nil
+| JsRecordRel_cons : forall (k: string) (vx vy: A) (xs xs' ys: js_record A),
+    rel vx vy -> JsRecordRel rel xs ys -> JsRecordAdd k vx xs xs' -> ~ JsRecordHasKey k ys -> JsRecordRel rel xs' ((k, vy) :: ys)%list
 .
 
 Inductive JsRecordNoDup {A: Type} : js_record A -> Prop :=
 | JsRecordNoDup_nil : JsRecordNoDup nil
 | JsRecordNoDup_cons : forall kx vx xs, JsRecordNoDup xs -> not (JsRecordHasKey kx xs) -> JsRecordNoDup ((kx, vx) :: xs)%list
+.
+
+Inductive JsRecordNoDupForall {A: Type} (P: A -> Prop): js_record A -> Prop :=
+| JsRecordNoDupForall_nil : JsRecordNoDupForall P nil
+| JsRecordNoDupForall_cons : forall kx vx xs, JsRecordNoDupForall P xs -> ~ JsRecordHasKey kx xs -> P vx -> JsRecordNoDupForall P ((kx, vx) :: xs)%list
 .
 
 Ltac rewrite_Forall_Exists_neg A key :=
@@ -122,6 +134,32 @@ Proof.
   intros; eapply proj2; eapply JsRecordHasKey_neg_Add; [exact H | exact H0].
 Qed.
 
+Theorem JsRecordHasKey_In: forall {A: Type} (key: string) (xs: js_record A),
+    JsRecordHasKey key xs <-> exists x, List.In (key, x) xs.
+Proof.
+  split; intros.
+  - induction H.
+    + destruct x as [kx vx]; subst; exists vx; simpl; left; reflexivity.
+    + destruct IHExists as [vx IHExists]; exists vx; simpl; right; exact IHExists.
+  - destruct H as [vx H]; destruct xs; [inv H |]; destruct p as [kx0 vx0]; simpl in H; destruct H.
+    + inv H; constructor; reflexivity.
+    + apply List.Exists_cons_tl; rewrite List.Exists_exists; exists (key, vx); split; [exact H | reflexivity].
+Qed.
+
+Theorem JsRecordHasKey_In0: forall {A: Type} (key: string) (x: A) (xs: js_record A),
+    List.In (key, x) xs -> JsRecordHasKey key xs.
+Proof.
+  intros; rewrite JsRecordHasKey_In; exists x; exact H.
+Qed.
+
+Theorem JsRecordHasKey_In_cons: forall {A: Type} (k: string) (vx vx0: A) (xs: js_record A),
+    List.In (k, vx) ((k, vx0) :: xs) ->
+    ~ JsRecordHasKey k xs ->
+    vx = vx0.
+Proof.
+  intros; inv H; [inv H1; reflexivity |]; rewrite JsRecordHasKey_In in H0; contradict H0; exists vx; exact H1.
+Qed.
+
 Lemma JsRecordNoDup_alt0 : forall {A: Type} (xs': js_record A),
   JsRecordNoDup xs' ->
   forall (kx: string) (vx: A) (xs: js_record A),
@@ -152,36 +190,33 @@ Proof.
   split; [eapply JsRecordNoDup_alt0 | eapply JsRecordNoDup_alt1]; [exact H | exact H0 | exact H | exact H0].
 Qed.
 
+Theorem JsRecordNoDupForall_alt : forall {A: Type} (P: A -> Prop) (xs: js_record A),
+    JsRecordNoDupForall P xs <-> JsRecordNoDup xs /\ JsRecordForall P xs.
+Proof.
+  split; intros.
+  - induction H; split; constructor; destruct IHJsRecordNoDupForall; simpl; assumption.
+  - induction xs; [| destruct a as [kx vx]]; constructor.
+    + apply IHxs; split_with H; inv H; assumption.
+    + apply proj1 in H; inv H; exact H4.
+    + apply proj2 in H; inv H; simpl in H2; exact H2.
+Qed.
+
 Theorem JsRecordAdd_not_nil : forall {A: Type} (kx: string) (vx: A) (xs: js_record A),
     not (JsRecordAdd kx vx xs nil).
 Proof.
   intros; intros H; inv H.
 Qed.
 
-Theorem JsRecordAdd_dec' : forall {A: Type} (kx: string) (xs': js_record A),
-    (exists vx xs, JsRecordAdd kx vx xs xs') \/ forall vx xs, not (JsRecordAdd kx vx xs xs').
-Proof.
-  intros; destruct (JsRecordHasKey_dec kx xs'); [left | right]; induction xs'.
-  - inv H.
-  - destruct a as [kx0 vx0]; destruct (string_dec kx0 kx).
-    + subst; exists vx0, xs'; apply JsRecordAdd_head.
-    + inv H; [contradiction n; reflexivity |]; specialize (IHxs' H1); destruct IHxs' as [vx1 [xs1 IHxs']]; exists vx1; exists ((kx0, vx0) :: xs1)%list; apply JsRecordAdd_cons; assumption.
-  - intros; intros H0; inv H0.
-  - intros; intros H0; destruct a as [kx0 vx0]; destruct (string_dec kx0 kx).
-    + subst; inv H0; [contradict H; apply List.Exists_cons_hd; reflexivity | contradiction H4; reflexivity].
-    + inv H0; [contradiction n; reflexivity |]; contradict H6; apply IHxs'; intros H0; contradict H; apply List.Exists_cons_tl; exact H0.
-Qed.
-
-Theorem JsRecordAdd_dec : forall {A: Type} (kx: string) (xs': js_record A),
-    (exists vx xs, JsRecordAdd kx vx xs xs') \/ not (exists vx xs, JsRecordAdd kx vx xs xs').
-Proof.
-  intros; destruct (JsRecordAdd_dec' kx xs'); [left; assumption | right]; intros H0; destruct H0 as [vx [xs H0]]; specialize (H vx xs); contradiction H.
-Qed.
-
 Theorem JsRecordAdd_HasKey : forall {A: Type} (kx: string) (vx: A) (xs xs': js_record A),
     JsRecordAdd kx vx xs xs' -> JsRecordHasKey kx xs'.
 Proof.
-  intros. induction H; [apply List.Exists_cons_hd; reflexivity | apply List.Exists_cons_tl; exact IHJsRecordAdd].
+  intros; induction H; [apply List.Exists_cons_hd; reflexivity | apply List.Exists_cons_tl; exact IHJsRecordAdd].
+Qed.
+
+Theorem JsRecordAdd_not_HasKey : forall {A: Type} (kx: string) (vx: A) (xs xs': js_record A),
+    JsRecordAdd kx vx xs xs' -> ~ JsRecordHasKey kx xs.
+Proof.
+  intros; induction H; [exact H |]; intros n; inv n; [contradiction H; reflexivity |]; contradiction IHJsRecordAdd.
 Qed.
 
 Theorem JsRecordAdd_ListAdd : forall {A: Type} (kx: string) (vx: A) (xs xs': js_record A),
@@ -198,12 +233,116 @@ Proof.
   - intros. specialize (H0 x). destruct x as [kx0 vx0]. simpl in *. apply H0. rewrite (List.Add_in H). simpl. right. exact H1.
 Qed.
 
-Theorem js_record_ind : forall {A: Type} (P: js_record A -> Prop),
-    P nil ->
-    (forall xs xs', P xs -> (exists kx vx, JsRecordAdd kx vx xs xs') -> P xs') ->
-    forall xs, P xs.
+Theorem JsRecordAdd_In : forall {A: Type} (kx: string) (vx: A) (xs xs': js_record A),
+    JsRecordAdd kx vx xs xs' -> List.In (kx, vx) xs'.
 Proof.
-  intros A P P0 Pn xs. induction xs; [exact P0 | apply (Pn xs); [exact IHxs |]]. destruct a as [kx vx]. exists kx. exists vx. apply JsRecordAdd_head.
+  intros; induction H; [left; reflexivity | right; exact IHJsRecordAdd].
+Qed.
+
+Theorem JsRecordAdd_is_cons : forall {A: Type} (kx: string) (vx vx': A) (xs xs': js_record A),
+    JsRecordAdd kx vx xs ((kx, vx') :: xs')%list -> vx = vx' /\ xs = xs'.
+Proof.
+  intros; inv H; [split; reflexivity | contradiction H3; reflexivity].
+Qed.
+
+Theorem JsRecordAdd_no_refl : forall {A: Type} (kx: string) (vx: A) (xs: js_record A),
+    ~ (JsRecordAdd kx vx xs xs).
+Proof.
+  intros; intros H; apply JsRecordAdd_ListAdd, List.Add_length in H; remember (Datatypes.length xs) as n; clear Heqn.
+  (* This should be automatic or trivial... *)
+  induction n; [discriminate H |]; inv H; exact (IHn H1).
+Qed.
+
+Theorem JsRecordAdd_no_head : forall {A: Type} (kx: string) (vx: A) (xs xs0: js_record A),
+    ~ (JsRecordAdd kx vx (xs0 ++ xs)%list xs).
+Proof.
+  intros; intros H; apply JsRecordAdd_ListAdd, List.Add_length in H; rewrite List.app_length in H;
+    remember (Datatypes.length xs) as n; remember (Datatypes.length xs0) as m; clear Heqn Heqm.
+  contradiction (Nat.succ_add_discr m n).
+Qed.
+
+Theorem JsRecordAdd_no_tail : forall {A: Type} (kx: string) (vx: A) (xs xs0: js_record A),
+    ~ (JsRecordAdd kx vx (xs ++ xs0)%list xs).
+Proof.
+  intros; intros H; apply JsRecordAdd_ListAdd, List.Add_length in H; rewrite List.app_length in H;
+    remember (Datatypes.length xs) as n; remember (Datatypes.length xs0) as m; clear Heqn Heqm; rewrite Nat.add_comm in H.
+  contradiction (Nat.succ_add_discr m n).
+Qed.
+
+Theorem JsRecordAdd_cons_hd : forall {A: Type} (kx kx': string) (vx vx': A) (xs xs': js_record A),
+    JsRecordAdd kx vx xs xs' -> JsRecordAdd kx vx ((kx', vx') :: xs) ((kx', vx') :: xs') \/ kx = kx'.
+Proof.
+  intros; destruct (string_dec kx kx'); [right; exact e | left; apply JsRecordAdd_cons; [intros n'; symmetry in n'; contradiction (n n') | exact H]].
+Qed.
+
+Theorem JsRecordAdd_List_Forall : forall {A: Type} (kx: string) (vx: A) (xs xs': js_record A),
+    JsRecordAdd kx vx xs xs' -> List.Forall (fun '(kx0, vx0) => vx = vx0 \/ kx0 <> kx) xs'.
+Proof.
+  intros; induction H; [| apply List.Forall_cons; [right; exact H | exact IHJsRecordAdd]].
+  apply List.Forall_cons; [left; reflexivity |]; rewrite JsRecordHasKey_neg in H; eapply List.Forall_impl; [| exact H]; intros; destruct a as [kx0 vx0]; right; intros n; symmetry in n; contradiction (H0 n).
+Qed.
+
+Theorem JsRecordAdd_In_once : forall {A: Type} (kx: string) (vx vx0: A) (xs xs': js_record A),
+    JsRecordAdd kx vx xs xs' -> List.In (kx, vx0) xs' -> vx = vx0.
+Proof.
+  intros. pose (JsRecordAdd_List_Forall H); rewrite List.Forall_forall in f; specialize (f _ H0); simpl in f; destruct f; [exact H1 | contradiction H1; reflexivity].
+Qed.
+
+Theorem JsRecordAdd_In_once' : forall {A: Type} (kx kx0: string) (vx vx0: A) (xs xs': js_record A),
+    JsRecordAdd kx vx xs xs' -> List.In (kx0, vx0) xs' -> kx <> kx0 <-> List.In (kx0, vx0) xs.
+Proof.
+  split; intros.
+  - induction H; simpl in H0; destruct H0; [inv H0; contradiction H1; reflexivity | exact H0 | inv H0; simpl; left; reflexivity | simpl; right; exact (IHJsRecordAdd H0)].
+  - destruct (string_dec kx kx0); [subst; exfalso | exact n]; rewrite (JsRecordAdd_In_once _ H H0) in H; apply JsRecordAdd_not_HasKey, JsRecordHasKey_neg in H; rewrite List.Forall_forall in H; specialize (H _ H1); simpl in H; contradiction H; reflexivity.
+Qed.
+
+Theorem JsRecordAdd_join_key: forall {A: Type} (kx: string) (vx vx0: A) (xs xs0 xs': js_record A),
+    JsRecordAdd kx vx xs xs' ->
+    JsRecordAdd kx vx0 xs0 xs' ->
+    vx = vx0.
+Proof.
+  intros; apply JsRecordAdd_In in H0; eapply JsRecordAdd_In_once in H; [exact H | exact H0].
+Qed.
+Ltac join_key_JsRecordAdd H H0 := remember (JsRecordAdd_join_key H H0) eqn:x; clear x; subst.
+
+Theorem JsRecordRel_eq_refl : forall {A: Type} (xs: js_record A), JsRecordNoDup xs -> JsRecordRel eq xs xs.
+Proof.
+  intros; induction xs; [| destruct a as [kx vx]]; econstructor; inv H; [reflexivity | apply IHxs | apply JsRecordAdd_head |]; assumption.
+Qed.
+
+Theorem JsRecordAdd_join_orig: forall {A: Type} (kx: string) (vx vx0: A) (xs xs0 xs': js_record A),
+    JsRecordNoDup xs' ->
+    JsRecordAdd kx vx xs xs' ->
+    JsRecordAdd kx vx0 xs0 xs' ->
+    JsRecordRel eq xs xs0.
+Proof.
+  intros; induction xs'; [inv H0 |]; destruct a as [kx' vx']; inv H H0 H1; [apply JsRecordRel_eq_refl; assumption | contradiction H5; reflexivity | contradiction H5; reflexivity |].
+  apply IHxs'; [exact H4 | ..].
+
+  destruct xs'; [inv H6 |]; destruct p as [kx'0 vx'0].
+  apply IHxs'.
+  - apply JsRecordAdd_cons.
+  f_equal; [exact (IHxs' H2 H3) |].
+  -
+Qed.
+Ltac join_key_JsRecordAdd H H0 := remember (JsRecordAdd_join_key H H0) eqn:x; clear x; subst.
+
+Theorem JsRecordRel_In: forall {A: Set} {rel: relation A} (k: string) (vx vy: A) (xs ys: js_record A),
+    JsRecordRel rel xs ys -> List.In (k, vx) xs -> List.In (k, vy) ys -> rel vx vy.
+Proof.
+  intros; induction H; [inv H1 |]; inv H3; destruct (string_dec k0 k); subst.
+  - apply JsRecordHasKey_In_cons in H1; [| exact H4]; apply JsRecordHasKey_In_cons in H0; [| exact H5]; subst; exact H.
+  - inv H0 H1; try (inv H3 + inv H0; contradiction n; reflexivity); exact (IHJsRecordRel H3 H0).
+  - apply JsRecordHasKey_In_cons in H1; [| exact H4]; inv H0; [inv H3; contradiction H5; reflexivity |]; rewrite (JsRecordAdd_In_once _ H6 H3) in *; exact H.
+  - inv H0 H1; try (inv H3 + inv H0; contradiction n; reflexivity).
+    + inv H3; apply IHJsRecordRel; [simpl; left; reflexivity | exact H0].
+    + pose (JsRecordAdd_In_once' _ _ H6 H3); apply i in n; apply IHJsRecordRel; [simpl; right; exact n | exact H0].
+Qed.
+
+Theorem JsRecordRel_add: forall {A: Set} {rel: relation A} (k: string) (vx vy: A) (xs xs' ys ys': js_record A),
+    JsRecordAdd k vx xs xs' -> JsRecordAdd k vy ys ys' -> JsRecordRel rel xs' ys' -> rel vx vy.
+Proof.
+  intros. apply JsRecordAdd_In in H, H0; eapply JsRecordRel_In in H1; [exact H1 | exact H | exact H0].
 Qed.
 
 Theorem JsRecordEqKeys_nil : forall {A: Type}, JsRecordEqKeys (@nil (string * A)) nil.
@@ -219,4 +358,12 @@ Qed.
 Theorem JsRecordEqKeys_not_nil_cons : forall {A: Type} (y: string * A) (ys: js_record A), ~JsRecordEqKeys nil (y :: ys)%list.
 Proof.
   intros. intros H. destruct y as [ky vy]. specialize (H ky). destruct H as [_ H]. assert_specialize H; [apply List.Exists_cons_hd; reflexivity |]. inv H.
+Qed.
+
+Theorem js_record_ind : forall {A: Type} (P: js_record A -> Prop),
+    P nil ->
+    (forall xs xs', P xs -> (exists kx vx, ~JsRecordHasKey kx xs -> JsRecordAdd kx vx xs xs') -> P xs') ->
+    forall xs, P xs.
+Proof.
+  intros A P P0 Pn xs. induction xs; [exact P0 | apply (Pn xs); [exact IHxs |]]. destruct a as [kx vx]. exists kx. exists vx. apply JsRecordAdd_head.
 Qed.
